generated-testcases/explicitPermutation/Frame001.bpl
@@ -242,6 +242,14 @@ function $ReachableFromParams#2($h:Heap, $x0,$x1:Ref, $a:Ref) : bool
    $ReachableFromParams#1($h, $x0, $a) || $ReachableFromParams#1($h, $x1, $a)
 }
 
+function $ReachableFromParams#4($h:Heap, $x0,$x1,$x2,$x3:Ref, $a:Ref) : bool
+{
+      $ReachableFromParams#1($h, $x0, $a) 
+   || $ReachableFromParams#1($h, $x1, $a)
+   || $ReachableFromParams#1($h, $x2, $a)
+   || $ReachableFromParams#1($h, $x3, $a)
+}
+
 /////////////////////////////////////////////////////////////////////////////
 // Extensional Equality
 function $Heap#Equal($h_1, $h_2:Heap) : bool
@@ -287,6 +295,22 @@ function $Heap#EqualFromParams#2($h_0:Heap, $x0_0,$x1_0:Ref, $h_1:Heap, $x0_1,$x
 {
     $Heap#EqualFromParams#1($h_0, $x0_0, $h_1, $x0_1) &&
     $Heap#EqualFromParams#1($h_0, $x1_0, $h_1, $x1_1)
+}
+
+function $Heap#EqualFromParams#4($h_0:Heap, $x0_0,$x1_0,$x2_0,$x3_0:Ref, $h_1:Heap, $x0_1,$x1_1,$x2_1,$x3_1:Ref) : bool 
+{
+    $Heap#EqualFromParams#1($h_0, $x0_0, $h_1, $x0_1) &&
+    $Heap#EqualFromParams#1($h_0, $x1_0, $h_1, $x1_1) &&
+    $Heap#EqualFromParams#1($h_0, $x2_0, $h_1, $x2_1) &&
+    $Heap#EqualFromParams#1($h_0, $x3_0, $h_1, $x3_1)
+}
+
+function $Heap#SameReachableFromParams#4($h_0:Heap, $x0_0,$x1_0,$x2_0,$x3_0:Ref, $h_1:Heap, $x0_1,$x1_1,$x2_1,$x3_1:Ref) : bool
+{
+	$Heap#SameReachableFromParams#1($h_0, $x0_0, $h_1, $x0_1) &&
+    $Heap#SameReachableFromParams#1($h_0, $x1_0, $h_1, $x1_1) &&
+    $Heap#SameReachableFromParams#1($h_0, $x2_0, $h_1, $x2_1) &&
+    $Heap#SameReachableFromParams#1($h_0, $x3_0, $h_1, $x3_1)
 }
 
 function $Heap#SameReachableFromParams#2($h_0:Heap, $x0_0,$x1_0:Ref, $h_1:Heap, $x0_1,$x1_1:Ref) : bool
@@ -526,30 +550,15 @@ procedure G_0($strategy:int, $h:Heap, $roots:Roots, x:Ref,y:Ref) returns ($h_0:H
 			assume $ReadObject($h_0, x);
 			y_0 := y ;
 			assume $ReadObject($h_0, y);
-			if(true )
-			{
-				$t#0_0 := $a#0_0 ;
-				assume $ReadObject($h_0, $a#0_0);
-			}
-			if(true )
-			{
-				z_0 := $t#0_0 ;
-				assume $ReadObject($h_0, $t#0_0);
-			}
-			if(true )
-			{
-				 call $h_0:=F_0(0, $h_0, $roots, x_0); 
-			}
-			if(true )
-			{
-				$t#1_0 := $Read($h_0,z_0,$field#v) ;
-				assume $ReadObject($h_0, z_0);
-				assume $ReadObject($h_0, $Read($h_0,z_0,$field#v) );
-			}
-			if(true )
-			{
-				$h_0:=$Write($h_0,y_0,$field#v,$t#1_0); assume $GoodHeap($h_0);
-			}
+			$t#0_0 := $a#0_0 ;
+			assume $ReadObject($h_0, $a#0_0);
+			z_0 := $t#0_0 ;
+			assume $ReadObject($h_0, $t#0_0);
+			 call $h_0:=F_0(0, $h_0, $roots, x_0); 
+			$t#1_0 := $Read($h_0,z_0,$field#v) ;
+			assume $ReadObject($h_0, z_0);
+			assume $ReadObject($h_0, $Read($h_0,z_0,$field#v) );
+			$h_0:=$Write($h_0,y_0,$field#v,$t#1_0); assume $GoodHeap($h_0);
 
 }
 
@@ -599,30 +608,15 @@ procedure G_1($strategy:int, $h:Heap, $roots:Roots, x:Ref,y:Ref) returns ($h_1:H
 			assume $ReadObject($h_1, x);
 			y_1 := y ;
 			assume $ReadObject($h_1, y);
-			if(true )
-			{
-				 call $h_1:=F_1(0, $h_1, $roots, x_1); 
-			}
-			if(true )
-			{
-				$t#0_1 := $a#0_1 ;
-				assume $ReadObject($h_1, $a#0_1);
-			}
-			if(true )
-			{
-				z_1 := $t#0_1 ;
-				assume $ReadObject($h_1, $t#0_1);
-			}
-			if(true )
-			{
-				$t#1_1 := $Read($h_1,z_1,$field#v) ;
-				assume $ReadObject($h_1, z_1);
-				assume $ReadObject($h_1, $Read($h_1,z_1,$field#v) );
-			}
-			if(true )
-			{
-				$h_1:=$Write($h_1,y_1,$field#v,$t#1_1); assume $GoodHeap($h_1);
-			}
+			 call $h_1:=F_1(0, $h_1, $roots, x_1); 
+			$t#0_1 := $a#0_1 ;
+			assume $ReadObject($h_1, $a#0_1);
+			z_1 := $t#0_1 ;
+			assume $ReadObject($h_1, $t#0_1);
+			$t#1_1 := $Read($h_1,z_1,$field#v) ;
+			assume $ReadObject($h_1, z_1);
+			assume $ReadObject($h_1, $Read($h_1,z_1,$field#v) );
+			$h_1:=$Write($h_1,y_1,$field#v,$t#1_1); assume $GoodHeap($h_1);
 
 }
 
@@ -727,60 +721,30 @@ procedure G_G($h:Heap, $roots:Roots, x:Ref,y:Ref)
 		    assume $ReadObject($h_0$0, x$0);
 		    y_0$0 := y$0 ;
 		    assume $ReadObject($h_0$0, y$0);
-		    if(true )
-		    {
-		    	$t#0_0$0 := $a#0_0$0 ;
-		    	assume $ReadObject($h_0$0, $a#0_0$0);
-		    }
-		    if(true )
-		    {
-		    	z_0$0 := $t#0_0$0 ;
-		    	assume $ReadObject($h_0$0, $t#0_0$0);
-		    }
-		    if(true )
-		    {
-		    	 call $h_0$0:=F_0(0, $h_0$0, $roots, x_0$0); 
-		    }
-		    if(true )
-		    {
-		    	$t#1_0$0 := $Read($h_0$0,z_0$0,$field#v) ;
-		    	assume $ReadObject($h_0$0, z_0$0);
-		    	assume $ReadObject($h_0$0, $Read($h_0$0,z_0$0,$field#v) );
-		    }
-		    if(true )
-		    {
-		    	$h_0$0:=$Write($h_0$0,y_0$0,$field#v,$t#1_0$0); assume $GoodHeap($h_0$0);
-		    }
+		    $t#0_0$0 := $a#0_0$0 ;
+		    assume $ReadObject($h_0$0, $a#0_0$0);
+		    z_0$0 := $t#0_0$0 ;
+		    assume $ReadObject($h_0$0, $t#0_0$0);
+		     call $h_0$0:=F_0(0, $h_0$0, $roots, x_0$0); 
+		    $t#1_0$0 := $Read($h_0$0,z_0$0,$field#v) ;
+		    assume $ReadObject($h_0$0, z_0$0);
+		    assume $ReadObject($h_0$0, $Read($h_0$0,z_0$0,$field#v) );
+		    $h_0$0:=$Write($h_0$0,y_0$0,$field#v,$t#1_0$0); assume $GoodHeap($h_0$0);
 
 		    // procedure body _1 start
 		    x_1$0 := x$0 ;
 		    assume $ReadObject($h_1$0, x$0);
 		    y_1$0 := y$0 ;
 		    assume $ReadObject($h_1$0, y$0);
-		    if(true )
-		    {
-		    	 call $h_1$0:=F_1(0, $h_1$0, $roots, x_1$0); 
-		    }
-		    if(true )
-		    {
-		    	$t#0_1$0 := $a#0_1$0 ;
-		    	assume $ReadObject($h_1$0, $a#0_1$0);
-		    }
-		    if(true )
-		    {
-		    	z_1$0 := $t#0_1$0 ;
-		    	assume $ReadObject($h_1$0, $t#0_1$0);
-		    }
-		    if(true )
-		    {
-		    	$t#1_1$0 := $Read($h_1$0,z_1$0,$field#v) ;
-		    	assume $ReadObject($h_1$0, z_1$0);
-		    	assume $ReadObject($h_1$0, $Read($h_1$0,z_1$0,$field#v) );
-		    }
-		    if(true )
-		    {
-		    	$h_1$0:=$Write($h_1$0,y_1$0,$field#v,$t#1_1$0); assume $GoodHeap($h_1$0);
-		    }
+		     call $h_1$0:=F_1(0, $h_1$0, $roots, x_1$0); 
+		    $t#0_1$0 := $a#0_1$0 ;
+		    assume $ReadObject($h_1$0, $a#0_1$0);
+		    z_1$0 := $t#0_1$0 ;
+		    assume $ReadObject($h_1$0, $t#0_1$0);
+		    $t#1_1$0 := $Read($h_1$0,z_1$0,$field#v) ;
+		    assume $ReadObject($h_1$0, z_1$0);
+		    assume $ReadObject($h_1$0, $Read($h_1$0,z_1$0,$field#v) );
+		    $h_1$0:=$Write($h_1$0,y_1$0,$field#v,$t#1_1$0); assume $GoodHeap($h_1$0);
 
 
 	assert 
